refactored eo_fin adequacy proof

fairness/lawyer/examples/eo_fin/eo_fin_adequacy.v
@@ -22,10 +22,6 @@ Section OblsAdequacy.
 
   Let M := AM2M ObligationsAM.
   
-  (* Definition obls_valid_evolution_step (c1 : cfg heap_lang) (oζ : olocale heap_lang)  *)
-  (*   (c2 : cfg heap_lang) (δ1 : mstate M) (ℓ : mlabel M) (δ2 : mstate M): Prop := *)
-  (*   obls_ves_wrapper c1 oζ c2 δ1 ℓ δ2.  *)
-
   Definition obls_st_rel (c: cfg heap_lang) (δ: mstate M) :=
     om_live_tids id locale_enabled c δ.
     
@@ -279,69 +275,28 @@ Section OblsAdequacy.
 
   Lemma obls_terminates_impl Σ
     {HEAP: heapGpreS Σ EM}
-    (extr : heap_lang_extrace) (e: expr)
+    (extr : heap_lang_extrace) (e: expr) (σ: state)
     (cps_degs: gmultiset Degree) (eb: nat)
-    (Hexfirst : (trfirst extr).1 = [e]):
-    (* (∀ tid, fair_ex tid extr) -> terminating_trace extr. *)
+    (s1 := init_om_state (trfirst extr) cps_degs eb (OP := OP))
+    (Hexfirst : trfirst extr = ([e], σ))
+    (WPe: forall (HEAP: heapGS Σ EM), ⊢ (([∗ map] l↦v ∈ heap σ, l ↦ v) ∗
+                                     (@em_init_resource heap_lang M EM Σ (@heap_fairnessGS Σ M EM HEAP) s1 tt))%I -∗
+            (WP e @locale_of [] e {{ _, @em_thread_post heap_lang M EM Σ (@heap_fairnessGS Σ M EM HEAP) 0 }})%I)
+    :
     extrace_fairly_terminating extr.
   Proof.
-    destruct (trfirst extr) as [tp_ σ1] eqn:EX0. simpl in *. subst tp_.
-
-    (* TODO: get rid of extra nat parameter of di *)
-    set (s1 := init_om_state (trfirst extr) cps_degs eb (OP := OP)).
-    
+    (* TODO: get rid of extra nat parameter of di *)    
     unshelve epose proof (simple_om_simulation_adequacy_terminate Σ NotStuck
                   _ _ _ _
-                  _ _ EX0) as FAIR_TERM; eauto.
+                  _ _ Hexfirst) as FAIR_TERM; eauto.
     { exact tt. }
-    { simpl. subst s1. rewrite EX0.
-      apply init_om_state_init. }
+    { simpl. subst s1. rewrite Hexfirst. apply init_om_state_init. }
     
     apply FAIR_TERM.
     red. intros ?. iStartProof. iIntros "[HEAP INIT] !>".
     iSplitL.
-    - simpl.
-      iApply (main_spec with "[-]").
-      4: { apply (phase_lt_fork π0 0). }
-      5: { simpl. iNext. iIntros (_) "X". iApply "X". }
-      3: { simpl. iIntros (? _) "X". iApply "X". }
-      { apply AMU_lift_top. }
-      { intros. rewrite /AMU_lift_MU__f.
-        rewrite -nclose_nroot.
-        apply AMU_lift_top. }
-      (* iFrame.  *)
-      rewrite /obls_init_resource. subst s1. simpl.
-      rewrite EX0.
-      
-      (* rewrite init_phases_helper.  *)
-      (* rewrite (init_phases_helper (start #0%nat #B) σ1). *)
-      pose proof (init_phases_helper (start #0%nat #B) σ1) as IP. rewrite IP.
-
-      rewrite locales_of_cfg_simpl. simpl.
-      rewrite union_empty_r_L. simpl.
-      iDestruct "INIT" as "(CPS & SIGS & OB & EPS & PH & EB)".
-      rewrite /cps_repr /sig_map_repr /eps_repr /obls_map_repr.
-      rewrite big_sepM_singleton.
-      rewrite fmap_empty.
-      rewrite !gset_to_gmap_singleton.
-      rewrite map_fmap_singleton.
-      iFrame.
-      rewrite mset_map_disj_union.
-      rewrite auth_frag_op.
-      iDestruct (own_op with "CPS") as "[CPS2 CPS0]".
-      iSplitL "CPS2".
-      + rewrite /cp_mul.
-        iApply (own_mono with "[$]").
-        apply auth_frag_mono.
-        rewrite mset_map_mul mset_map_singleton.
-        apply gmultiset.gmultiset_included.
-        apply scalar_mul_le. lia.
-      + iApply (own_mono with "CPS0").
-        apply auth_frag_mono.
-        rewrite mset_map_mul mset_map_singleton.
-        apply gmultiset.gmultiset_included.
-        apply scalar_mul_le. lia.
-    - subst s1. rewrite EX0. iApply om_sim_RAH.
+    - iApply WPe. iFrame. 
+    - subst s1. rewrite Hexfirst. iApply om_sim_RAH.
   Qed.
 
 End OblsAdequacy.
@@ -356,179 +311,6 @@ Section EOFinAdequacy.
   Let OM := ObligationsModel. 
   Let M := AM2M ObligationsAM. 
   
-  Definition eofin_valid_evolution_step (c1 : cfg heap_lang) (oζ : olocale heap_lang) 
-    (c2 : cfg heap_lang) (δ1 : mstate M) (ℓ : mlabel M) (δ2 : mstate M): Prop :=
-    obls_ves_wrapper c1 oζ c2 δ1 ℓ δ2. 
-
-  Definition eofin_st_rel (c: cfg heap_lang) (δ: mstate M) :=
-    om_live_tids id locale_enabled c δ. 
-    
-  Definition eofin_sim_rel (extr: execution_trace heap_lang) (omtr: auxiliary_trace M) :=
-    valid_state_evolution_fairness eofin_valid_evolution_step extr omtr ∧
-    eofin_st_rel (trace_last extr) (trace_last omtr).
-
-  Definition eofin_om_traces_match: extrace heap_lang -> trace (mstate M) (mlabel M) -> Prop :=
-    traces_match
-      (fun oτ '(_, τ') => oτ = τ')
-      eofin_st_rel
-      locale_step
-      (@mtrans M).
-
-  Lemma eofin_sim_rel_FB: rel_finitary eofin_sim_rel.
-  Proof using.
-    clear. red. intros extr mtr [tp' σ'] oζ. 
-    simpl. rewrite /eofin_sim_rel. simpl.
-    rewrite /eofin_valid_evolution_step /eofin_st_rel. simpl.
-    apply list_approx_smaller_card. 
-    apply @OM_fin_branch_impl; by apply _.
-  Qed. 
-    
-  Theorem om_simulation_adequacy_model_trace Σ
-        `{hPre: !heapGpreS Σ EM} (s: stuckness)
-        (e1: expr) σ1 (s1: mstate M) p
-        (INIT: em_is_init_st ([e1], σ1) s1 (ExecutionModel := EM))
-        (extr : heap_lang_extrace)
-        (Hvex : extrace_valid extr)
-        (Hexfirst : trfirst extr = ([e1], σ1))    :
-    wp_premise Σ s e1 σ1 s1 eofin_sim_rel (p: @em_init_param _ _ EM) ->
-    ∃ (omtr: trace (mstate M) (mlabel M)), 
-      eofin_om_traces_match extr omtr ∧
-      trfirst omtr = s1.
-  Proof using.
-    (* clear H1 H0 H.  *)
-    intros (* FIN *) PREM.
-
-    unshelve epose proof (@strong_simulation_adequacy_traces _ _ _ hPre s e1 σ1
-                s1
-                eofin_sim_rel
-                p
-                extr
-                Hvex
-                ltac:(done)
-                eofin_valid_evolution_step
-                eofin_st_rel
-                (fun oτ '(_, τ') => oτ = τ')
-                _ _ _ _ _ _ _
-      ) as SIM.
-    { simpl. intros ????[??]? STEP.
-      red in STEP. simpl in STEP. destruct STEP as [STEP ->].
-      destruct o; [| done].
-      simpl in STEP. red in STEP. apply STEP. }
-    { simpl. intros ????[??]? STEP.
-      red in STEP. simpl in STEP. destruct STEP as [STEP ->].
-      destruct o; [| done].  
-      simpl in STEP. red in STEP.
-      constructor. apply STEP. }
-    { simpl. intros ?? SIM. apply SIM. }
-    { simpl. intros ?? SIM. apply SIM. }
-    { apply eofin_sim_rel_FB. }
-    { done. }
-    { done. }
-    done. 
-  Qed.
-
-  Lemma eofin_matching_traces_termination extr mtr
-    (VALID: extrace_valid extr)
-    (OM_WF0: om_st_wf (trfirst mtr))
-    (FAIR: ∀ tid, fair_ex tid extr)
-    (MATCH: eofin_om_traces_match extr mtr)
-    :
-  terminating_trace extr.
-  Proof using.
-    clear -MATCH FAIR VALID OM OM_WF0.
-    assert (exists omtr, traces_match (fun ℓ τ => ℓ.2 = Some τ) eq (@mtrans M) (@mtrans OM) mtr omtr) as [omtr MATCHo]. 
-    { clear -MATCH mtr.
-      exists (project_nested_trace id ((mbind Some) ∘ snd) mtr).
-      eapply trace_utils.traces_match_impl. 
-      3: { eapply nested_trace_construction.
-           - eapply traces_match_valid2; eauto. 
-           - simpl. intros. simpl.
-             rewrite /step_label_matches. destruct res.
-             destruct o as [[[??]?]|]. 
-             2: { right. red. eauto. }
-             left. do 3 eexists. split; [reflexivity| ]. simpl.
-             destruct o; [done| ].
-             apply traces_match_valid2 in MATCH.
-             eapply trace_valid_steps' in H; eauto. inversion H. 
-           - intros. destruct ℓ. simpl in H0. destruct o; [| done].
-             simpl in H0. inversion H0. subst. simpl.
-             inversion H. subst. eauto. }
-      2: done.
-      simpl. intros [??] ?. simpl. destruct o; done. }
-
-    
-    pose proof (traces_match_compose _ _ _ MATCH MATCHo) as MATCH'.
-
-    (* TODO: extract these lemmas *)
-    assert (out_om_traces_match locale_step Some
-              (fun oτ c => from_option (fun τ => locale_enabled τ c) False oτ)
-              extr omtr) as MATCH''.
-    { eapply trace_utils.traces_match_impl; [..| apply MATCH'].
-      - simpl. intros ?? ([??] & <- & ?). done.
-      - simpl. intros ?? (? & ? & ?). subst. eauto. } 
-    assert (∀ ζ, out_fair (λ oτ c,
-                     from_option (λ τ, locale_enabled τ c) False oτ) ζ extr) as FAIR''.
-    { intros oζ. red. simpl. clear -FAIR.
-      apply fair_by_equiv. red. intros n EN. simpl in EN.
-      destruct (extr S!! n) eqn:NTH; rewrite NTH in EN; [| done]. 
-      simpl in EN. 
-      destruct oζ as [ζ | ]; [| done]. 
-      simpl in EN. simpl.
-      specialize (FAIR ζ). apply fair_by_equiv in FAIR.
-      red in FAIR. specialize (FAIR n ltac:(by rewrite NTH)).
-      destruct FAIR as (?&?&?&FAIR).
-      do 2 eexists. split; eauto.
-      destruct FAIR as [| FAIR]. 
-      { left. done. }
-      right. destruct FAIR as (?&?&?). eauto. }
-    pose proof (out_om_fairness_preserved _ _ _ _ extr omtr MATCH'' FAIR'') as OM_FAIR. 
-
-    pose proof (traces_match_valid2 _ _ _ _ _ _ MATCH'') as OM_VALID.  
-    pose proof (obls_fair_trace_terminate _ OM_VALID OM_FAIR) as OM_TERM.
-    specialize_full OM_TERM.
-    { intros. eapply pres_by_valid_trace with (i := 0) (j := i) in OM_VALID. 
-      2: apply wf_preserved_by_loc_step.
-      2: apply wf_preserved_by_fork_step.
-      2: { rewrite state_lookup_0. simpl.
-           apply traces_match_first in MATCHo.
-           by rewrite -MATCHo. }
-      2: lia.
-      by rewrite H in OM_VALID. }
-    { apply fin_wf. }
-    { apply fin_wf. }
-    
-    pose proof (traces_match_preserves_termination _ _ _ _ _ _ MATCH'' OM_TERM). 
-    done.
-  Qed. 
-  
-  
-  Theorem simple_om_simulation_adequacy_terminate Σ
-        (* `{hPre: !heapGpreS Σ EM} (s: stuckness) *)
-        (* (e1: expr) σ1 (s1: mstate OM) (* p *) *)
-        (* (INIT: obls_is_init_st OP ([e1], σ1) s1) *)
-        (* (extr : heap_lang_extrace) *)
-        (* (Hexfirst : trfirst extr = ([e1], σ1))    : *)
-        `{hPre: !heapGpreS Σ EM} (s: stuckness)
-        (e1: expr) σ1 (s1: mstate M) p
-        (INIT: em_is_init_st ([e1], σ1) s1 (ExecutionModel := EM))
-        (extr : heap_lang_extrace)
-        (* (Hvex : extrace_valid extr) *)
-        (Hexfirst : trfirst extr = ([e1], σ1)):
-    (* rel_finitary (sim_rel LM) → *)
-    wp_premise Σ s e1 σ1 s1 eofin_sim_rel (p: @em_init_param _ _ EM) -> 
-    extrace_fairly_terminating extr.
-  Proof.
-    rewrite /extrace_fairly_terminating.
-    intros (* Hterm Hfb *) Hwp (* VALID *) VALID FAIR.
-
-    destruct (om_simulation_adequacy_model_trace
-                Σ _ e1 _ s1 _ INIT _ VALID Hexfirst Hwp) as (omtr&MATCH&OM0).
-
-    eapply eofin_matching_traces_termination; eauto.
-    rewrite OM0.
-    simpl in INIT. red in INIT. set_solver. 
-  Qed.
-
   (* TODO: move *)
   Definition sig_mapΣ := #[GFunctor $ authUR (gmapUR nat (agreeR SignalId))].
   Global Instance subG_sig_mapΣ {Σ}: subG sig_mapΣ Σ → SigMapPreG Σ.
@@ -543,171 +325,98 @@ Section EOFinAdequacy.
   Global Instance subG_eofinΣ {Σ}: subG eofinΣ Σ → EoFinPreG Σ.
   Proof. solve_inG. Qed.
 
+  Definition obls_init_resource' `{!ObligationsGS Σ}
+    (δ: mstate OM) (_: unit): iProp Σ :=
+    ([∗ mset] '(π, d) ∈ (ps_cps δ), cp π d) ∗    
+    own obls_sigs (◯ (sig_map_repr $ ps_sigs δ)) ∗
+    own obls_obls (◯ (obls_map_repr $ ps_obls δ)) ∗
+    own obls_eps (◯ (eps_repr $ ps_eps δ)) ∗
+    ([∗ map] τ↦π ∈ ps_phases δ, th_phase_eq τ π) ∗
+    exc_lb (ps_exc_bound δ)
+  .
+  Lemma obls_init_resource'_WIP `{!ObligationsGS Σ} δ p:
+    obls_init_resource δ p = obls_init_resource' δ p.
+  Proof using. Admitted.
+
   (* TODO: move *)
-  Lemma om_live_tids_init e σ ds eb:
-      om_live_tids id locale_enabled ([e], σ) (init_om_state ([e], σ) ds eb).
-  Proof using. 
-    red. intros ?.
-    rewrite /has_obls. simpl. 
-    rewrite locales_of_cfg_simpl. simpl. rewrite union_empty_r_L.
-    rewrite gset_to_gmap_singleton. 
-    destruct (decide (ζ = 0)) as [-> | ?].
-    2: { simpl. simpl. rewrite lookup_singleton_ne; [| done]. done. }
-    by rewrite lookup_singleton.
+  Lemma cp_mul_alt `{oGS: !ObligationsGS Σ} π d n:
+    cp_mul π d n (oGS := oGS) ⊣⊢ ([∗ mset] '(π, d) ∈ (n *: {[+ (π, d) +]}), cp π d (oGS := oGS)).
+  Proof using.
+    rewrite obligations_resources.cp_mul_unseal. rewrite /obligations_resources.cp_mul_def.
+    iInduction n as [| n] "IH".
+    { set_solver. }
+    simpl. rewrite gmultiset_scalar_mul_S_l big_sepMS_disj_union.
+    rewrite big_sepMS_singleton.
+    iSplit; iIntros "[??]"; iFrame; by iApply "IH".
   Qed.
 
-  Lemma no_obls_live_tids
-          {Hinv: @heapGS eofinΣ M EM}
-          (oGS := @heap_fairnessGS eofinΣ _ _ Hinv)
-    (tp : list expr)
-  (σ : state)
-  (δ' : ProgressState)
-  ee
-  (TH_OWN : threads_own_obls (tp, σ) δ'):
-  gen_heap_interp (heap σ) -∗ obls_msi δ' (oGS := oGS) -∗
-  cur_posts tp ee (λ _ : val, obls 0 ∅ (oGS := oGS)) -∗
-  ⌜om_live_tids id locale_enabled (tp, σ) δ'⌝.
-  Proof using.
-    clear -Hinv TH_OWN.
-    iIntros "HEAP MSI POSTS".
-    rewrite /om_live_tids. iIntros (τ OBτ).
-    rewrite /locale_enabled.
-    red in OBτ.
-    destruct (ps_obls δ' !! τ) as [V| ] eqn:OB_; [| done].
-    simpl in OBτ.
-    red in TH_OWN. rewrite set_eq in TH_OWN. specialize (TH_OWN τ).
-    apply proj2 in TH_OWN. specialize (TH_OWN ltac:(eapply elem_of_dom; eauto)).
-    apply locales_of_cfg_Some in TH_OWN as [e Ee]. simpl in Ee.
-    iExists _. iSplit; [done| ].
-    destruct (language.to_val e) eqn:VALe; [| done].
-    apply from_locale_lookup in Ee.
-    iDestruct (posts_of_empty_mapping with "[POSTS]") as "foo"; eauto.
-    simpl.
-    iDestruct (obls_msi_exact with "MSI foo") as %?.
-    clear -OB_ OBτ H. rewrite OB_ in H. congruence.
-  Qed. 
-
-  (* TODO: generalize? move? *)
-  Lemma om_sim_RAH 
-    {Hinv: @heapGS eofinΣ M EM}
-    σ1 e ds eb:
-  ⊢
-  rel_always_holds0 
-    (@eofin_sim_rel) NotStuck
-    (@state_interp heap_lang _ eofinΣ _)
-    (λ _ : language.val heap_lang,
-       @em_thread_post heap_lang _ _ eofinΣ
-         (@heap_fairnessGS eofinΣ
-            _
-            _ Hinv) 0) e σ1
-    (@init_om_state _ _ _ 10 OP ([e], σ1) ds eb).
-  Proof using.
-    rewrite /rel_always_holds0.
-    
-    iIntros (extr omtr [tp σ] VALID EX0 OM0 EX_FIN CONT_SIM).
-    simpl. iIntros (NSTUCK FOOBAR).
-    iIntros "(%VALID_STEP & HEAP & MSI & [%TH_OWN %OBLS]) POSTS".
-    
-    iApply fupd_mask_intro_discard; [done| ].
-    
-    clear CONT_SIM. 
-
-    destruct extr.
-    { iPureIntro.  
-      simpl in VALID_STEP.
-      inversion VALID. subst. 
-      red in EX0, OM0. simpl in EX0, OM0. subst.
-      rewrite /eofin_sim_rel. rewrite /valid_state_evolution_fairness /om_live_tids.
-      split; [done| ]. simpl. red.
-      apply om_live_tids_init. }
- 
-    simpl in VALID_STEP. inversion VALID. subst. simpl in *.
-    red in EX_FIN. simpl in EX_FIN. subst. simpl.
-    rewrite /eofin_sim_rel. iSplit.
-    { simpl. iPureIntro. red. 
-      destruct ℓ. done. }
-    simpl. rewrite /eofin_st_rel.
-
-    iApply (no_obls_live_tids with "[$] [$] [$]"). done.  
-  Qed.
+  (* TODO: move, replace original *)
+    Lemma cp_mul_weaken `{oGS: ObligationsGS Σ} π1 π2 deg n1 n2
+      (PH_LE: phase_le π1 π2)
+      (LE: n2 <= n1):
+      cp_mul π1 deg n1 (oGS := oGS) -∗ cp_mul π2 deg n2 (oGS := oGS).
+    Proof using.
+      iIntros "CPS".
+      apply Nat.le_sum in LE as [? ->].
+      iDestruct (cp_mul_split with "CPS") as "[CPS _]".
+      rewrite obligations_resources.cp_mul_unseal.
+      iInduction n2 as [| n] "IH".
+      { set_solver. }
+      simpl. iDestruct "CPS" as "[CP CPS]". iSplitL "CP".
+      { by iApply cp_weaken. }
+      by iApply "IH".
+    Qed.
 
   Lemma eofin_terminates_impl
     (extr : heap_lang_extrace)
-    (Hexfirst : (trfirst extr).1 = [start #(0%nat) #B]):
-    (* (∀ tid, fair_ex tid extr) -> terminating_trace extr. *)
+    (START: trfirst extr = ([start #(0%nat) #B], Build_state ∅ ∅)):
     extrace_fairly_terminating extr. 
   Proof.
     assert (heapGpreS eofinΣ EM) as HPreG.
     { apply _. }
 
-    destruct (trfirst extr) as [tp_ σ1] eqn:EX0. simpl in *. subst tp_.
+    eapply @obls_terminates_impl with
+      (cps_degs := (2 * B + 5) *: {[+ d2 B +]} ⊎ 50 *: {[+ d0 B +]})
+      (eb := 20); eauto.
+    1-5: by apply _.
+    1-2: by apply fin_wf.
+    Unshelve. 2-6: by apply _.
 
-    (* TODO: get rid of extra nat parameter of di *)
-    set (s1 := init_om_state (trfirst extr)
-               ((2 * B + 5) *: {[+ d2 B +]} ⊎ 50 *: {[+ d0 B +]})
-                 20
-        ). 
+    iIntros (?) "[HEAP INIT]".
+    iApply (main_spec with "[-]").
+    5: { simpl. iNext. iIntros (_) "X". iApply "X". }
+    3: { simpl. iIntros (? _) "X". iApply "X". }
+    { apply AMU_lift_top. }
+    { intros. rewrite /AMU_lift_MU__f.
+      rewrite -nclose_nroot.
+      apply AMU_lift_top. }
     
-    unshelve epose proof (simple_om_simulation_adequacy_terminate eofinΣ NotStuck
-                  _ _ _ _
-                  _ _ EX0) as FAIR_TERM; eauto.
-    { exact tt. }
-    { simpl. subst s1. rewrite EX0.
-      apply init_om_state_init. }
-    
-    apply FAIR_TERM.
-    red. intros ?. iStartProof. iIntros "[HEAP INIT] !>".
-    iSplitL.
-    - simpl. 
-      iApply (main_spec with "[-]").
-      4: { apply (phase_lt_fork π0 0). }
-      5: { simpl. iNext. iIntros (_) "X". iApply "X". }
-      3: { simpl. iIntros (? _) "X". iApply "X". }
-      { apply AMU_lift_top. }
-      { intros. rewrite /AMU_lift_MU__f.
-        rewrite -nclose_nroot.
-        apply AMU_lift_top. }
-      (* iFrame.  *)
-      rewrite /obls_init_resource. subst s1. simpl.
-      rewrite EX0.
+    simpl. rewrite START.
+    rewrite obls_init_resource'_WIP. 
+    rewrite /obls_init_resource' /init_om_state. 
       
-      (* rewrite init_phases_helper.  *)
-      (* rewrite (init_phases_helper (start #0%nat #B) σ1). *)
-      pose proof (init_phases_helper (start #0%nat #B) σ1) as IP. rewrite IP. 
-
-      rewrite locales_of_cfg_simpl. simpl.
-      rewrite union_empty_r_L. simpl. 
-      iDestruct "INIT" as "(CPS & SIGS & OB & EPS & PH & EB)".
-      rewrite /cps_repr /sig_map_repr /eps_repr /obls_map_repr.
-      rewrite big_sepM_singleton. 
-      rewrite fmap_empty.
-      rewrite !gset_to_gmap_singleton. 
-      rewrite map_fmap_singleton.      
-      iFrame.
-      rewrite mset_map_disj_union.
-      rewrite auth_frag_op.
-      iDestruct (own_op with "CPS") as "[CPS2 CPS0]".
-      iSplitL "CPS2".
-      + rewrite /cp_mul.
-        iApply (own_mono with "[$]").
-        apply auth_frag_mono.
-        rewrite mset_map_mul mset_map_singleton.
-        apply gmultiset.gmultiset_included. 
-        apply scalar_mul_le. lia.
-      + iApply (own_mono with "CPS0").
-        apply auth_frag_mono.
-        rewrite mset_map_mul mset_map_singleton.
-        apply gmultiset.gmultiset_included. 
-        apply scalar_mul_le. lia.
-    - subst s1. rewrite EX0. iApply om_sim_RAH. 
-  Qed.
+    rewrite init_phases_helper.
+    rewrite locales_of_cfg_simpl. simpl.
+    rewrite union_empty_r_L.
+    iDestruct "INIT" as "(CPS & SIGS & OB & EPS & PH & EB)".
+    rewrite /cps_repr /sig_map_repr /eps_repr /obls_map_repr. 
+    rewrite big_sepM_singleton. 
+    rewrite fmap_empty.
+    rewrite !gset_to_gmap_singleton. 
+    rewrite map_fmap_singleton.      
+    iFrame.
+    rewrite mset_map_disj_union. rewrite big_sepMS_disj_union.
+    rewrite !mset_map_mul !mset_map_singleton.
+    rewrite -!cp_mul_alt. iDestruct "CPS" as "[CPS2 CPS0]".
+    iSplitL "CPS2"; (iApply cp_mul_weaken; [..| by iFrame]; [apply phase_lt_fork | lia]).
+  Qed. 
 
 End EOFinAdequacy.
 
 Theorem eofin_terminates (N: nat):
   forall extr,
-    (trfirst extr).1 = [start #0%nat #N] → 
+    trfirst extr = ([start #(0%nat) #N], Build_state ∅ ∅) ->
     extrace_fairly_terminating extr.
 Proof using.
-  intros. eapply eofin_terminates_impl; eauto.
+  intros. eapply eofin_terminates_impl; eauto.  
 Qed.
